gates/repo.ts
@@ -39,6 +39,7 @@ allow("LICENSE", 4000);
 allow("flake.nix", 1500);
 allow("bend2/base.bend", 32000);
 allow("bend2/bend.lean", 400000);
+allow("bend2/bang.lean", 10000);
 allow("bend2/bend.ts", 44000);
 allow("bend2/comp.ts", 64000);
 allow("bend2/main.ts", 10000);
